split proof and specs into local and global components

src/Examples/DistributedCtr/DistCtrImpl_Global.v
@@ -1,26 +1,9 @@
 From iris.algebra Require Import auth frac_auth excl.
 From iris.base_logic.lib Require Import invariants.
 From iris.heap_lang Require Import proofmode notation lib.par lib.spin_lock.
+Require Import DistributedCtr.Helpers.
+Require Import DistributedCtr.DistCtrImpl_Local.
 
-(* LOCAL NODE-BASED FUNCTIONS *)
-Definition alloc_node: val := λ: "()",
-  let: "node" := ref (SOME #0) in
-  let: "lk" := newlock #() in
-  Pair "node" "lk".
-
-Definition update_node: val := 
-  λ: "node",
-  match: !"node" with
-    SOME "v1" => "node" <- SOME ("v1" + #1);;
-                        #1
-  | NONE => #0
-  end.
-
-Definition kill_node: val :=
-  λ: "node",
-  "node" <- NONE.
-
-(* GLOBAL, CLIENT-FACING FUNCTIONS *)
 Definition alloc_replicas : val := λ: "()",
   let: "master" := alloc_node #() in
   let: "backup" := alloc_node #() in
@@ -71,38 +54,6 @@ Definition update_replicas: val :=
 
 Section proof.
   Context `{!heapG Σ, !spawnG Σ, !lockG Σ, !inG Σ (authR (optionUR (exclR ZO)))}.
-  Definition LockN : namespace := nroot .@ "LockN".
-
-  Lemma ghost_var_alloc n :
-    (|==> ∃ γ, own γ (● (Excl' n)) ∗ own γ (◯ (Excl' n)))%I.
-  Proof.
-    iMod (own_alloc (● (Excl' n) ⋅ ◯ (Excl' n))) as (γ) "[??]".
-    - by apply auth_both_valid.
-    - by eauto with iFrame.
-  Qed.
-
-  Lemma ghost_var_agree γ n m :
-    own γ (● (Excl' n)) -∗ own γ (◯ (Excl' m)) -∗ ⌜ n = m ⌝. Proof. iIntros "Hγ● Hγ◯".
-    Check own_valid_2.
-    by iDestruct (own_valid_2 with "Hγ● Hγ◯")
-      as %[<-%Excl_included%leibniz_equiv _]%auth_both_valid.
-  Qed.
-
-  Lemma ghost_var_update γ n' n m :
-    own γ (● (Excl' n)) -∗ own γ (◯ (Excl' m)) ==∗
-      own γ (● (Excl' n')) ∗ own γ (◯ (Excl' n')).
-  Proof.
-    iIntros "Hγ● Hγ◯".
-    iMod (own_update_2 _ _ _ (● Excl' n' ⋅ ◯ Excl' n') with "Hγ● Hγ◯") as "[$$]".
-    { apply auth_update. apply option_local_update. apply exclusive_local_update. done. }
-    done.
-  Qed.
-
-  Definition node_val_inv (n : Z) (optv: option Z) (γ : gname): iProp Σ := 
-      ⌜ optv = Some n ∨ optv = None ⌝ ∗ own γ (◯ (Excl' n)).
-
-  Definition node_lock_inv (γ: gname) : iProp Σ :=
-    (∃ n, own γ (● (Excl' n)))%I.
 
   Definition global_inv_unlocked (optv1 optv2: option Z) (γ1 γ2 γ3 γ4: gname) (lk1 lk2 : val): iProp Σ :=
     is_lock LockN γ3 lk1 (node_lock_inv γ1)
@@ -116,30 +67,6 @@ Section proof.
     ∗ (∃ n, (node_val_inv n optv1 γ1))
     ∗ (∃ n, (node_val_inv n optv2 γ2)).
   (* Notes: loc = kind of like a Coq literal number, LitV (LitLoc loc) is an actual value in the language *)
-
-  Lemma alloc_node_spec : 
-    {{{ True%I }}}
-      alloc_node #()
-      {{{ r1 lk γ γ1 , RET PairV r1 lk;
-          is_lock LockN γ lk (node_lock_inv γ1) ∗
-          node_val_inv 0 (Some 0) γ1
-    }}}.
-  Proof.
-    iIntros (Φ) "_ HPost".
-    iMod (ghost_var_alloc 0) as (γ1) "[Hγ1● Hγ1◯]".
-
-    unfold alloc_node.
-    wp_alloc master as "Hr1".
-    wp_let.
- 
-    wp_apply (newlock_spec LockN (node_lock_inv γ1) with "[- Hγ1◯ Hr1 HPost]").
-    iExists 0; auto.
-    iIntros (lk γ) "HIsLk".
-    wp_let.
-    wp_pures.
-    iApply "HPost". 
-    iFrame; auto.
-  Qed.
 
   Lemma alloc_replicas_spec : 
     {{{ True%I }}}
@@ -164,59 +91,6 @@ Section proof.
     unfold global_inv_unlocked; unfold node_val_inv.
     iSplitL "Hnodeinv1"; iExists 0; iFrame; auto.
   Qed.
-
-  Lemma update_node_some_spec : ∀ (n: Z) γ1 node,
-      {{{
-           node ↦ SOMEV #n
-           ∗ node_lock_inv γ1
-           ∗ node_val_inv n (Some n) γ1
-    }}}
-      update_node #node
-    {{{ RET #1;
-          node ↦ SOMEV #(n+1)
-          ∗ node_lock_inv γ1
-          ∗ node_val_inv (n+1) (Some (n+1)) γ1
-    }}}.
-  Proof.
-    iIntros (n γ1 node Φ) "(Hnode & Hlkinv & Hnodeinv & Hown) HPost".
-    unfold update_node.
-    unfold node_lock_inv.
-    iDestruct "Hlkinv" as (n') "Hlkinv".
-    iMod (ghost_var_update γ1 (n+1) with "Hlkinv Hown") as "[Hγ1● Hγ1◯]".
-    wp_pures.
-    wp_load.
-    wp_pures.
-    wp_store.
-    iApply "HPost". 
-    iFrame; auto.
-  Qed.
-
-  Lemma update_node_none_spec : ∀ (n: Z) γ1 node,
-      {{{
-           node ↦ NONEV
-           ∗ node_lock_inv γ1
-           ∗ node_val_inv n None γ1
-    }}}
-      update_node #node
-    {{{ RET #0;
-          node ↦ NONEV
-          ∗ node_lock_inv γ1
-          ∗ (∃ n, node_val_inv n None γ1)
-    }}}.
-  Proof.
-    iIntros (n γ1 node Φ) "(Hnode & Hlkinv & Hnodeinv & Hown) HPost".
-    unfold update_node.
-    unfold node_lock_inv.
-    iDestruct "Hlkinv" as (n') "Hlkinv".
-    wp_pures.
-    wp_load.
-    wp_pures.
-    iApply "HPost".
-    iSplitL "Hnode"; auto.
-    iSplitL "Hlkinv". iExists n'; auto.
-    unfold node_val_inv. iExists n. iSplit; auto. 
-  Qed.
-
   Lemma recover_replicas_both_alive_spec : ∀ (n: Z) γ1 γ2 node1 node2,
       {{{
           ⌜ ~n < 0 ⌝
