src/Examples/DistributedCtr/DistCtrImpl_Local.v
@@ -1,0 +1,108 @@
+From iris.algebra Require Import auth frac_auth excl.
+From iris.base_logic.lib Require Import invariants.
+From iris.heap_lang Require Import proofmode notation lib.par lib.spin_lock.
+Require Import DistributedCtr.Helpers.
+
+(* LOCAL NODE-BASED FUNCTIONS *)
+Definition alloc_node: val := λ: "()",
+  let: "node" := ref (SOME #0) in
+  let: "lk" := newlock #() in
+  Pair "node" "lk".
+
+Definition update_node: val := 
+  λ: "node",
+  match: !"node" with
+    SOME "v1" => "node" <- SOME ("v1" + #1);;
+                        #1
+  | NONE => #0
+  end.
+
+Definition kill_node: val :=
+  λ: "node",
+  "node" <- NONE.
+
+Section proof.
+  Context `{!heapG Σ, !spawnG Σ, !lockG Σ, !inG Σ (authR (optionUR (exclR ZO)))}.
+
+  Definition node_val_inv (n : Z) (optv: option Z) (γ : gname): iProp Σ := 
+      ⌜ optv = Some n ∨ optv = None ⌝ ∗ own γ (◯ (Excl' n)).
+
+  Definition node_lock_inv (γ: gname) : iProp Σ :=
+    (∃ n, own γ (● (Excl' n)))%I.
+
+  Lemma alloc_node_spec : 
+    {{{ True%I }}}
+      alloc_node #()
+      {{{ r1 lk γ γ1 , RET PairV r1 lk;
+          is_lock LockN γ lk (node_lock_inv γ1) ∗
+          node_val_inv 0 (Some 0) γ1
+    }}}.
+  Proof.
+    iIntros (Φ) "_ HPost".
+    iMod (ghost_var_alloc 0) as (γ1) "[Hγ1● Hγ1◯]".
+
+    unfold alloc_node.
+    wp_alloc master as "Hr1".
+    wp_let.
+ 
+    wp_apply (newlock_spec LockN (node_lock_inv γ1) with "[- Hγ1◯ Hr1 HPost]").
+    iExists 0; auto.
+    iIntros (lk γ) "HIsLk".
+    wp_let.
+    wp_pures.
+    iApply "HPost". 
+    iFrame; auto.
+  Qed.
+
+  Lemma update_node_some_spec : ∀ (n: Z) γ1 node,
+      {{{
+           node ↦ SOMEV #n
+           ∗ node_lock_inv γ1
+           ∗ node_val_inv n (Some n) γ1
+    }}}
+      update_node #node
+    {{{ RET #1;
+          node ↦ SOMEV #(n+1)
+          ∗ node_lock_inv γ1
+          ∗ node_val_inv (n+1) (Some (n+1)) γ1
+    }}}.
+  Proof.
+    iIntros (n γ1 node Φ) "(Hnode & Hlkinv & Hnodeinv & Hown) HPost".
+    unfold update_node.
+    unfold node_lock_inv.
+    iDestruct "Hlkinv" as (n') "Hlkinv".
+    iMod (ghost_var_update γ1 (n+1) with "Hlkinv Hown") as "[Hγ1● Hγ1◯]".
+    wp_pures.
+    wp_load.
+    wp_pures.
+    wp_store.
+    iApply "HPost". 
+    iFrame; auto.
+  Qed.
+
+  Lemma update_node_none_spec : ∀ (n: Z) γ1 node,
+      {{{
+           node ↦ NONEV
+           ∗ node_lock_inv γ1
+           ∗ node_val_inv n None γ1
+    }}}
+      update_node #node
+    {{{ RET #0;
+          node ↦ NONEV
+          ∗ node_lock_inv γ1
+          ∗ (∃ n, node_val_inv n None γ1)
+    }}}.
+  Proof.
+    iIntros (n γ1 node Φ) "(Hnode & Hlkinv & Hnodeinv & Hown) HPost".
+    unfold update_node.
+    unfold node_lock_inv.
+    iDestruct "Hlkinv" as (n') "Hlkinv".
+    wp_pures.
+    wp_load.
+    wp_pures.
+    iApply "HPost".
+    iSplitL "Hnode"; auto.
+    iSplitL "Hlkinv". iExists n'; auto.
+    unfold node_val_inv. iExists n. iSplit; auto. 
+  Qed.
+End proof.
