src/Examples/DistributedCtr/Helpers.v
@@ -1,0 +1,33 @@
+From iris.algebra Require Import auth frac_auth excl.
+From iris.base_logic.lib Require Import invariants.
+From iris.heap_lang Require Import proofmode notation lib.par lib.spin_lock.
+
+Section proof.
+  Context `{!heapG Σ, !spawnG Σ, !lockG Σ, !inG Σ (authR (optionUR (exclR ZO)))}.
+  Definition LockN : namespace := nroot .@ "LockN".
+
+  Lemma ghost_var_alloc n :
+    (|==> ∃ γ, own γ (● (Excl' n)) ∗ own γ (◯ (Excl' n)))%I.
+  Proof.
+    iMod (own_alloc (● (Excl' n) ⋅ ◯ (Excl' n))) as (γ) "[??]".
+    - by apply auth_both_valid.
+    - by eauto with iFrame.
+  Qed.
+
+  Lemma ghost_var_agree γ n m :
+    own γ (● (Excl' n)) -∗ own γ (◯ (Excl' m)) -∗ ⌜ n = m ⌝. Proof. iIntros "Hγ● Hγ◯".
+    Check own_valid_2.
+    by iDestruct (own_valid_2 with "Hγ● Hγ◯")
+      as %[<-%Excl_included%leibniz_equiv _]%auth_both_valid.
+  Qed.
+
+  Lemma ghost_var_update γ n' n m :
+    own γ (● (Excl' n)) -∗ own γ (◯ (Excl' m)) ==∗
+      own γ (● (Excl' n')) ∗ own γ (◯ (Excl' n')).
+  Proof.
+    iIntros "Hγ● Hγ◯".
+    iMod (own_update_2 _ _ _ (● Excl' n' ⋅ ◯ Excl' n') with "Hγ● Hγ◯") as "[$$]".
+    { apply auth_update. apply option_local_update. apply exclusive_local_update. done. }
+    done.
+  Qed.
+End proof.
